TODO.md
@@ -15,3 +15,5 @@
 
 - When writing spec, the reads/writes of mappings (and likely arrays too) should happen in the 
   order they appear in the bytecode. Otherwise, we may need ta add keccak axioms.
+
+- Optimizations on vs off
